abstract_integers.v
@@ -1,0 +1,301 @@
+(* Copyright (c) 2012, Robbert Krebbers. *)
+(* This file is distributed under the terms of the BSD license. *)
+(** This file describes an axiomatization of machine integers. It differs
+in two important aspects from the specification in the C11 standard. *)
+
+(** First of all, the C standard allows sign-and-magnitude, ones' complement,
+and two's complement representations for signed integers. However, this design
+dates back to the seventies (when machines using such representations actually
+existed) and is hardly of any relevance today (all machines use two's
+complement). Although our axiomatization does not explicitly enforce a two's
+complement representation, any implementation has to be in order to give
+an efficient implementation of our axiomatization of bitwise operations
+(and [&], or [|], xor [^], and complement [~]). *)
+
+(** We describe all operations, including bitwise operations, by their
+translation to mathematical integers, so as to make the axiomatization more
+uniform. The C standard, on the other hand, specifies bitwise operations using
+the values of individual bits (and is quite unclear whether padding bits should
+be taken into account), and uses mathematical values for all other operations.
+In spire of our restriction to two's complement, we still allow multiple integer
+representations for the same integer from any type apart from unsigned char.
+Hence, an implementation is allowed to include padding bits. *)
+
+(** Also, we attempt to be fairly minimal, and thereby also allow certain
+implementations than are forbidden by the C standard. For example, we only
+require two integer types to be present (unsigned char, and signed int), and
+do not put restrictions on the range of these integer types. In future work we
+may define a more restricted axiomatization that is a proper subclass of the
+implementations allowed by the C standard. *)
+Require Export prelude.
+
+(** * Operations *)
+(** We define inductive data types [unop] and [binop] describing the operations
+that can be performed on integers, and give denotations using mathematical
+integers. These denotations are used in the axiomatization to describe the
+operations on machine integers. *)
+Inductive unop :=
+  | NegOp | ComplOp.
+Inductive comp_kind :=
+  | CEq | CLt | CLe.
+Inductive binop :=
+  | PlusOp | MinusOp | MultOp
+  | ShiftLOp | ShiftROp
+  | AndOp | OrOp | XorOp
+  | DivOp | ModOp
+  | CompOp : comp_kind → binop.
+Notation EqOp := (CompOp CEq).
+Notation LtOp := (CompOp CLt).
+Notation LeOp := (CompOp CLe).
+
+Instance unop_dec (op1 op2 : unop) : Decision (op1 = op2).
+Proof. solve_decision. Defined.
+Instance comp_kind_dec (c1 c2 : comp_kind) : Decision (c1 = c2).
+Proof. solve_decision. Defined.
+Instance binop_dec (op1 op2 : binop) : Decision (op1 = op2).
+Proof. solve_decision. Defined.
+
+Definition Z_eval_unop (op : unop) (x : Z) : Z :=
+  match op with
+  | NegOp => -x
+  | ComplOp => Z.lnot x
+  end%Z.
+
+Definition Z_comp (c : comp_kind) : Z → Z → Prop :=
+  match c with
+  | CEq => (=)
+  | CLt => (<)
+  | CLe => (≤)
+  end%Z.
+Instance Z_comp_dec c : ∀ x y, Decision (Z_comp c x y) :=
+  match c return ∀ x y : Z, Decision (Z_comp c x y) with
+  | CEq => decide_rel (=)
+  | CLt => decide_rel (<)
+  | CLe => decide_rel (≤)
+  end%Z.
+
+Definition nat_comp (c : comp_kind) : nat → nat → Prop :=
+  match c with
+  | CEq => (=)
+  | CLt => (<)
+  | CLe => (≤)
+  end.
+Instance nat_comp_dec c : ∀ x y, Decision (nat_comp c x y) :=
+  match c return ∀ x y : nat, Decision (nat_comp c x y) with
+  | CEq => decide_rel (=)
+  | CLt => decide_rel (<)
+  | CLe => decide_rel (≤)
+  end.
+
+Definition Z_eval_binop (x2m : Z) (op : binop) (x1 x2 : Z) : option Z :=
+  match op with
+  | PlusOp => Some (x1 + x2)
+  | MinusOp => Some (x1 - x2)
+  | MultOp => Some (x1 * x2)
+  | ShiftLOp => guard (0 ≤ x1); guard (0 ≤ x2 < x2m); Some (Z.shiftl x1 x2)
+  | ShiftROp => guard (0 ≤ x1); guard (0 ≤ x2 < x2m); Some (Z.shiftr x1 x2)
+  | AndOp => Some (Z.land x1 x2)
+  | OrOp => Some (Z.lor x1 x2)
+  | XorOp => Some (Z.lxor x1 x2)
+  | DivOp => guard (x2 ≠ 0); Some (x1 `quot` x2)
+  | ModOp => guard (x2 ≠ 0); Some (x1 `rem` x2)
+  | CompOp c => Some (Z_of_sumbool (decide_rel (Z_comp c) x1 x2))
+  end%Z.
+
+(** We consider both signed and unsigned integers. Signed integers are an
+interval between [-x] (included) and [x] of mathematical integers.
+Similarly, unsigned integers are an interval between [0] (included) and [2 * x]
+of mathematical integers. *)
+Inductive signedness := Signed | Unsigned.
+Instance signedness_eq_dec (s1 s2 : signedness) : Decision (s1 = s2).
+Proof. solve_decision. Defined.
+
+(** * The required operations on machine integers *)
+(** The axiomatization of machine integers is parametrized by two data types:
+- [Ti] represents the set of integer types, and,
+- [Vi] represents the set of integer values.
+
+We require various operations to be implemented on these data types. *)
+Class IntEnv (Ti Vi : Set) := {
+  int_type_size : Ti → nat;
+  int_type_sign : Ti → signedness;
+  int_type_range : Ti → Z;
+  type_of_int : Vi → Ti;
+  TuChar : Ti;
+  TuChar_bits : nat;
+  TsInt : Ti;
+  char := { x | type_of_int x = TuChar };
+  encode_int : Vi → listset (list char);
+  decode_int : Ti → list char → option Vi;
+  int_to_Z : Vi → Z;
+  int_of_Z : Ti → Z → Vi;
+  int_eval_unop : unop → Vi → option Vi;
+  int_eval_binop : binop → Vi → Vi → option Vi;
+  int_cast : Ti → Vi → option Vi
+}.
+
+Arguments int_type_size _ _ _ _ : simpl never.
+Arguments int_type_sign _ _ _ _ : simpl never.
+Arguments int_type_range _ _ _ _ : simpl never.
+Arguments type_of_int _ _ _ _ : simpl never.
+Arguments TuChar _ _ _ : simpl never.
+Arguments TuChar_bits _ _ _ : simpl never.
+Arguments TsInt _ _ _ : simpl never.
+Arguments char _ _ {_} : clear implicits.
+Arguments encode_int _ _ _ _ : simpl never.
+Arguments decode_int _ _ _ _ _ : simpl never.
+Arguments int_to_Z _ _ _ _ : simpl never.
+Arguments int_of_Z _ _ _ _ _ : simpl never.
+Arguments int_eval_unop _ _ _ _ _ : simpl never.
+Arguments int_eval_binop _ _ _ _ _ _ : simpl never.
+Arguments int_cast _ _ _ _ _ : simpl never.
+
+Definition int_type_lower `{IntEnv Ti Vi} (τ : Ti) : Z :=
+  match int_type_sign τ with
+  | Signed => -int_type_range τ
+  | Unsigned => 0
+  end%Z.
+Definition int_type_upper `{IntEnv Ti Vi} (τ : Ti) : Z :=
+  match int_type_sign τ with
+  | Signed => int_type_range τ
+  | Unsigned => 2 * int_type_range τ
+  end%Z.
+Definition int_type_bits `{IntEnv Ti Vi} (τ : Ti) : nat :=
+  int_type_size τ * TuChar_bits.
+
+Definition int_sign `{IntEnv Ti Vi} : Vi → signedness :=
+  int_type_sign ∘ type_of_int.
+Definition int_lower `{IntEnv Ti Vi} : Vi → Z :=
+  int_type_lower ∘ type_of_int.
+Definition int_upper `{IntEnv Ti Vi} : Vi → Z :=
+  int_type_upper ∘ type_of_int.
+
+Definition maybe_int_of_Z `{IntEnv Ti Vi} (τ : Ti) (x : Z) : option Vi :=
+  guard (int_type_lower τ ≤ x ≤ int_type_upper τ)%Z;
+  Some (int_of_Z τ x).
+Definition int_true `{IntEnv Ti Vi} : Vi := int_of_Z TsInt 1.
+Definition int_false `{IntEnv Ti Vi} : Vi := int_of_Z TsInt 0.
+Definition int_of_sumbool `{IntEnv Ti Vi} {P Q} (p : {P} + {Q}) : Vi :=
+  (if p then int_true else int_false)%Z.
+
+(** * The axiomatization of machine integers *)
+(** The following class defines the laws that an implementation of machine
+integers should satisfy. Most of these laws are straightforward. Keep in mind,
+that like the C standard, overflow of unsigned integers is defined behavior
+(namely, it wraps modulo), whereas overflow of signed integers is undefined
+behavior. As [int_eval_unop], [int_eval_binop], and [int_cast], are partial
+functions, an implementation is thus free to decide whether to yield a bogus
+values, or to make the result actual undefined behavior. *)
+Class IntEnvSpec Ti Vi `{IntEnv Ti Vi}
+    `{∀ τ1 τ2 : Ti, Decision (τ1 = τ2)}
+    `{∀ x1 x2 : Vi, Decision (x1 = x2)} := {
+  int_type_range_pos τ :
+    (0 < int_type_range τ)%Z;
+  size_TuChar :
+    int_type_size TuChar = 1;
+  sign_TuChar :
+    int_type_sign TuChar = Unsigned;
+  range_TuChar :
+    (2 * int_type_range TuChar = 2 ^ TuChar_bits)%Z;
+  int_type_size_enough (τ : Ti) :
+    (2 * int_type_range τ ≤ 2 ^ int_type_bits τ)%Z;
+
+  encode_int_exists x :
+    ∃ cs, cs ∈ encode_int x;
+  encode_int_length x cs :
+    cs ∈ encode_int x →
+    length cs = int_type_size (type_of_int x);
+  decode_int_typed τ cs x :
+    decode_int τ cs = Some x →
+    type_of_int x = τ;
+  decode_encode_int τ cs x :
+    decode_int τ cs = Some x →
+    cs ∈ encode_int x;
+  encode_decode_int (cs : list (char Ti Vi)) x :
+    cs ∈ encode_int x →
+    decode_int (type_of_int x) cs = Some x;
+  decode_int_zeros τ c :
+    int_to_Z (`c) = 0%Z →
+    decode_int τ (replicate (int_type_size τ) c) = Some (int_of_Z τ 0);
+
+  int_to_Z_in_range x :
+    (int_lower x ≤ int_to_Z x < int_upper x)%Z;
+  int_of_Z_typed τ x :
+    type_of_int (int_of_Z τ x) = τ;
+  int_of_to_Z x :
+    int_of_Z (type_of_int x) (int_to_Z x) = x;
+  int_to_of_Z_signed τ x :
+    int_type_sign τ = Signed →
+    (int_type_lower τ ≤ x < int_type_upper τ)%Z →
+    int_to_Z (int_of_Z τ x) = x;
+  int_to_of_Z_unsigned τ x :
+    int_type_sign τ = Unsigned →
+    int_to_Z (int_of_Z τ x) = (x `mod` int_type_upper τ)%Z;
+
+  int_unop_typed op x τ y :
+    int_eval_unop op x = Some y →
+    type_of_int x = τ →
+    type_of_int y = τ;
+  int_unop_signed op x τ :
+    type_of_int x = τ →
+    int_type_sign τ = Signed →
+    (int_type_lower τ ≤ Z_eval_unop op (int_to_Z x) < int_type_upper τ)%Z →
+    int_eval_unop op x = Some (int_of_Z τ (Z_eval_unop op (int_to_Z x)));
+  int_unop_unsigned op x τ :
+    type_of_int x = τ →
+    int_type_sign τ = Unsigned →
+    int_eval_unop op x = Some (int_of_Z τ (Z_eval_unop op (int_to_Z x)));
+
+  int_binop_typed op x1 x2 τ y :
+    int_eval_binop op x1 x2 = Some y →
+    type_of_int x1 = τ →
+    type_of_int x2 = τ →
+    type_of_int y = τ;
+  int_binop_signed op x1 x2 τ y :
+    Z_eval_binop (int_type_bits τ) op (int_to_Z x1) (int_to_Z x2) = Some y →
+    type_of_int x1 = τ →
+    type_of_int x2 = τ →
+    int_type_sign τ = Signed →
+    (int_type_lower τ ≤ y < int_type_upper τ)%Z →
+    int_eval_binop op x1 x2 = Some (int_of_Z τ y);
+  int_binop_unsigned op x1 x2 τ y :
+    Z_eval_binop (int_type_bits τ) op (int_to_Z x1) (int_to_Z x2) = Some y →
+    type_of_int x1 = τ →
+    type_of_int x2 = τ →
+    int_type_sign τ = Unsigned →
+    int_eval_binop op x1 x2 = Some (int_of_Z τ y);
+
+  int_cast_typed τ x y :
+    int_cast τ x = Some y →
+    type_of_int y = τ;
+  int_cast_signed τ x :
+    int_type_sign τ = Signed →
+    (int_type_lower τ ≤ int_to_Z x < int_type_upper τ)%Z →
+    int_cast τ x = Some (int_of_Z τ (int_to_Z x));
+  int_cast_unsigned τ x :
+    int_type_sign τ = Unsigned →
+    int_cast τ x = Some (int_of_Z τ (int_to_Z x))
+}.
+
+(** * Theorems *)
+(** Some derived properties. *)
+Section abstract_integers.
+  Context `{IntEnvSpec Ti Vi}.
+
+  Lemma int_type_size_ne_0 τ : int_type_size τ ≠ 0.
+  Proof.
+    intros Hτ. eapply Zlt_not_le, (int_type_size_enough τ).
+    unfold int_type_bits. rewrite Hτ, mult_0_l, Z.pow_0_r.
+    pose proof (int_type_range_pos τ). lia.
+  Qed.
+  Lemma int_type_size_pos τ :
+    (0 < int_type_size τ)%Z.
+  Proof. pose proof (int_type_size_ne_0 τ). lia. Qed.
+
+  Lemma decode_int_nil τ : decode_int τ [] = None.
+  Proof.
+    destruct (decode_int τ []) eqn:E; [|done].
+    apply decode_encode_int, encode_int_length in E.
+    by destruct (int_type_size_ne_0 (type_of_int v)).
+  Qed.
+End abstract_integers.
